formic_site_duct/db.dfy
@@ -313,4 +313,5 @@ module DB {
       ops := operations;
     }
   }
+
 }
